lifting.v
@@ -31,17 +31,9 @@ Lemma wp_alloc_pst E σ n Φ :
              ownP σ' ={E}=★ Φ (LitV $ LitLoc l))
   ⊢ WP Alloc (Lit $ LitInt n) @ E {{ Φ }}.
 Proof.
-  iIntros {?}  "[HP HΦ]".
-  set (φ (e' : expr []) σ' ef := ∃ l,
-          ef = None ∧ e' = Lit (LitLoc l) ∧
-          (∀ m, σ !! (shift_loc l m) = None) ∧
-          (∃ vl, n = length vl ∧ init_mem l vl σ = σ')).
-  iApply (wp_lift_atomic_head_step _ φ σ);
-    try (by simpl; eauto).
-  { intros; subst φ; inv_head_step; eauto 8. }
-  iFrame "HP". iNext. iIntros {v2 σ2 ef} "[Hφ HP]".
-  iDestruct "Hφ" as %(l & -> & [= <-]%of_to_val_flip & ? & ?); simpl.
-  rewrite right_id. iApply "HΦ". auto.
+  iIntros {?}  "[HP HΦ]". iApply (wp_lift_atomic_head_step _ σ); eauto.
+  iFrame "HP". iNext. iIntros {v2 σ2 ef} "[% HP]". inv_head_step.
+  rewrite right_id. iApply "HΦ". iFrame. eauto.
 Qed.
 
 Lemma wp_free_pst E σ l n Φ :
@@ -51,33 +43,26 @@ Lemma wp_free_pst E σ l n Φ :
   ▷ (ownP (free_mem l (Z.to_nat n) σ) ={E}=★ Φ (LitV $ LitUnit))
   ⊢ WP Free (Lit $ LitInt n) (Lit $ LitLoc l) @ E {{ Φ }}.
 Proof.
-  iIntros {??}  "[HP HΦ]".
-  set (φ (e' : expr []) σ' ef :=
-          ef = None ∧ e' = Lit LitUnit ∧ σ' = free_mem l (Z.to_nat n) σ).
-  iApply (wp_lift_atomic_head_step _ φ σ); try (by simpl; eauto).
-  { intros; subst φ; inv_head_step; eauto. }
-  iFrame "HP". iNext. iIntros {v2 σ2 ef} "[Hφ HP]".
-  iDestruct "Hφ" as %(-> & [= <-]%of_to_val_flip & ->); simpl.
-  iSplit; last done. iApply ("HΦ" with "HP").
+  iIntros {??}  "[HP HΦ]". iApply (wp_lift_atomic_head_step _ σ); eauto.
+  iFrame "HP". iNext. iIntros {v2 σ2 ef} "[% HP]". inv_head_step.
+  rewrite right_id. by iApply "HΦ".
 Qed.
 
 Lemma wp_read_sc_pst E σ l n v Φ :
   σ !! l = Some (RSt n, v) →
   ▷ ownP σ ★ ▷ (ownP σ ={E}=★ Φ v) ⊢ WP Read ScOrd (Lit $ LitLoc l) @ E {{ Φ }}.
 Proof.
-  intros. rewrite -(wp_lift_atomic_det_head_step σ v σ None) ?right_id //.
-  intros; inv_head_step; eauto using to_of_val.
+  iIntros {?} "[??]". iApply wp_lift_atomic_det_head_step; eauto.
+  by intros; inv_head_step; eauto using to_of_val. by rewrite right_id; iFrame.
 Qed.
 
 Lemma wp_read_in_pst E σ l n v Φ :
   σ !! l = Some(RSt $ S n, v) →
   ▷ ownP σ ★ ▷ (ownP (<[l:=(RSt n, v)]>σ) ={E}=★ Φ v)
-  ⊢ WP Read InOrd (Lit $ LitLoc l) @ E {{ Φ }}.
+  ⊢ WP Read Na2Ord (Lit $ LitLoc l) @ E {{ Φ }}.
 Proof.
-  intros.
-  rewrite -(wp_lift_atomic_det_head_step σ v (<[l:=(RSt n, v)]>σ) None)
-          ?right_id //.
-  intros; inv_head_step; eauto using to_of_val.
+  iIntros {?} "[??]". iApply wp_lift_atomic_det_head_step; eauto.
+  by intros; inv_head_step; eauto using to_of_val. by rewrite right_id; iFrame.
 Qed.
 
 Lemma wp_read_na_pst E1 E2 l Φ :
@@ -85,8 +70,8 @@ Lemma wp_read_na_pst E1 E2 l Φ :
   (|={E1,E2}=> ∃ σ n v, σ !! l = Some(RSt $ n, v) ∧
      ▷ ownP σ ★
      ▷ (ownP (<[l:=(RSt $ S n, v)]>σ) ={E2,E1}=★
-          WP Read InOrd (Lit $ LitLoc l) @ E1 {{ Φ }}))
-  ⊢ WP Read NaOrd (Lit $ LitLoc l) @ E1 {{ Φ }}.
+          WP Read Na2Ord (Lit $ LitLoc l) @ E1 {{ Φ }}))
+  ⊢ WP Read Na1Ord (Lit $ LitLoc l) @ E1 {{ Φ }}.
 Proof.
   iIntros {?} "HΦP". iApply (wp_lift_head_step E1 E2); auto.
   iPvs "HΦP" as {σ n v} "(%&HΦ&HP)"; first set_solver. iPvsIntro.
@@ -100,22 +85,18 @@ Lemma wp_write_sc_pst E σ l e v v' Φ :
   ▷ ownP σ ★ ▷ (ownP (<[l:=(RSt 0, v)]>σ) ={E}=★ Φ (LitV LitUnit))
   ⊢ WP Write ScOrd (Lit $ LitLoc l) e @ E {{ Φ }}.
 Proof.
-  intros.
-  rewrite-(wp_lift_atomic_det_head_step σ (LitV LitUnit)
-             (<[l:=(RSt 0, v)]>σ) None) ?right_id //=. eauto.
-  intros; inv_head_step; eauto.
+  iIntros {??} "[??]". iApply wp_lift_atomic_det_head_step; simpl; eauto.
+  by intros; inv_head_step; eauto. by rewrite right_id; iFrame.
 Qed.
 
 Lemma wp_write_in_pst E σ l e v v' Φ :
   to_val e = Some v →
   σ !! l = Some(WSt, v') →
   ▷ ownP σ ★ ▷ (ownP (<[l:=(RSt 0, v)]>σ) ={E}=★ Φ (LitV LitUnit))
-  ⊢ WP Write InOrd (Lit $ LitLoc l) e @ E {{ Φ }}.
+  ⊢ WP Write Na2Ord (Lit $ LitLoc l) e @ E {{ Φ }}.
 Proof.
-  intros.
-  rewrite-(wp_lift_atomic_det_head_step σ (LitV LitUnit)
-             (<[l:=(RSt 0, v)]>σ) None) ?right_id //=. eauto.
-  intros; inv_head_step; eauto.
+  iIntros {??} "[??]". iApply wp_lift_atomic_det_head_step; simpl; eauto.
+  by intros; inv_head_step; eauto. by rewrite right_id; iFrame.
 Qed.
 
 Lemma wp_write_na_pst E1 E2 l e v Φ :
@@ -124,8 +105,8 @@ Lemma wp_write_na_pst E1 E2 l e v Φ :
   (|={E1,E2}=> ∃ σ v', σ !! l = Some(RSt 0, v') ∧
      ▷ ownP σ ★
      ▷ (ownP (<[l:=(WSt, v')]>σ) ={E2,E1}=★
-       WP Write InOrd (Lit $ LitLoc l) e @ E1 {{ Φ }}))
-  ⊢ WP Write NaOrd (Lit $ LitLoc l) e @ E1 {{ Φ }}.
+       WP Write Na2Ord (Lit $ LitLoc l) e @ E1 {{ Φ }}))
+  ⊢ WP Write Na1Ord (Lit $ LitLoc l) e @ E1 {{ Φ }}.
 Proof.
   iIntros {??} "HΦP".
   iApply (wp_lift_head_step E1 E2); auto.
@@ -134,34 +115,38 @@ Proof.
   inv_head_step. rewrite right_id. iApply ("HP" with "HΦ").
 Qed.
 
-Lemma wp_cas_fail_pst E σ l n z1 z2 z' Φ :
-  σ !! l = Some (RSt n, LitV $ LitInt z') → z' ≠ z1 →
+Lemma wp_cas_fail_pst E σ l n e1 v1 e2 v2 vl Φ :
+  to_val e1 = Some v1 → to_val e2 = Some v2 →
+  σ !! l = Some (RSt n, vl) →
+  value_eq σ v1 vl = Some false →
   ▷ ownP σ ★ ▷ (ownP σ ={E}=★ Φ (LitV $ LitInt 0))
-  ⊢ WP CAS (Lit $ LitLoc l) (Lit $ LitInt z1) (Lit $ LitInt z2) @ E {{ Φ }}.
+  ⊢ WP CAS (Lit $ LitLoc l) e1 e2 @ E {{ Φ }}.
 Proof.
-  intros.
-  rewrite-(wp_lift_atomic_det_head_step σ (LitV $ LitInt 0) σ None) ?right_id //.
-  intros; inv_head_step; eauto.
+  iIntros {????} "[HP HΦ]".
+  iApply wp_lift_atomic_det_head_step; try by simpl; eauto 10.
+    by intros; inv_head_step; eauto.
+  iFrame. iNext. by rewrite right_id.
 Qed.
 
-Lemma wp_cas_suc_pst E σ l z1 z2 Φ :
-  σ !! l = Some (RSt 0, LitV $ LitInt z1) →
-  ▷ ownP σ ★ ▷ (ownP (<[l:=(RSt 0, LitV $ LitInt z2)]>σ) ={E}=★ Φ (LitV $ LitInt 1))
-  ⊢ WP CAS (Lit $ LitLoc l) (Lit $ LitInt z1) (Lit $ LitInt z2) @ E {{ Φ }}.
+Lemma wp_cas_suc_pst E σ l e1 v1 e2 v2 vl Φ :
+  to_val e1 = Some v1 → to_val e2 = Some v2 →
+  σ !! l = Some (RSt 0, vl) →
+  value_eq σ v1 vl = Some true →
+  ▷ ownP σ ★ ▷ (ownP (<[l:=(RSt 0, v2)]>σ) ={E}=★ Φ (LitV $ LitInt 1))
+  ⊢ WP CAS (Lit $ LitLoc l) e1 e2 @ E {{ Φ }}.
 Proof.
-  intros.
-  rewrite -(wp_lift_atomic_det_head_step σ (LitV $ LitInt 1)
-              (<[l:=(RSt 0, LitV $ LitInt z2 )]>σ) None) ?right_id //.
-  intros; inv_head_step; eauto.
+  iIntros {????} "[HP HΦ]".
+  iApply wp_lift_atomic_det_head_step; try by simpl; eauto 10.
+    by intros; inv_head_step; eauto.
+  iFrame. iNext. by rewrite right_id.
 Qed.
 
 (** Base axioms for core primitives of the language: Stateless reductions *)
 Lemma wp_fork E e Φ :
   ▷ Φ (LitV LitUnit) ★ ▷ WP e {{ _, True }} ⊢ WP Fork e @ E {{ Φ }}.
 Proof.
-  rewrite -(wp_lift_pure_det_head_step (Fork e) (Lit LitUnit) (Some e)) //=.
-  rewrite later_sep -(wp_value _ _ (Lit _)) //.
-  intros; inv_head_step; eauto.
+  iIntros "[??]". iApply wp_lift_pure_det_head_step; eauto.
+  by intros; inv_head_step; eauto. iNext. iFrame. by iApply wp_value.
 Qed.
 
 Lemma wp_rec E f xl erec erec' e el Φ :
@@ -170,18 +155,16 @@ Lemma wp_rec E f xl erec erec' e el Φ :
   subst_l xl el erec = Some erec' →
   ▷ WP subst f e erec' @ E {{ Φ }} ⊢ WP App e el @ E {{ Φ }}.
 Proof.
-  intros -> ??.
-  rewrite-(wp_lift_pure_det_head_step (App _ _) (subst f (Rec f xl erec) erec') None)
-          ?right_id //=.
-  intros; inv_head_step; eauto.
+  iIntros {???} "?". iApply wp_lift_pure_det_head_step; subst; eauto.
+  by intros; inv_head_step; eauto. iNext. by iFrame.
 Qed.
 
 Lemma wp_bin_op E op l1 l2 l' Φ :
   bin_op_eval op l1 l2 = Some l' →
   ▷ Φ (LitV l') ⊢ WP BinOp op (Lit l1) (Lit l2) @ E {{ Φ }}.
 Proof.
-  intros Heval. rewrite -(wp_lift_pure_det_head_step (BinOp op _ _) (Lit l') None)
-    ?right_id -?wp_value //; intros; inv_head_step; eauto.
+  iIntros {?} "?". iApply wp_lift_pure_det_head_step; eauto.
+  by intros; inv_head_step; eauto. iNext. rewrite right_id. by iApply wp_value.
 Qed.
 
 Lemma wp_case E i e el Φ :
@@ -189,7 +172,7 @@ Lemma wp_case E i e el Φ :
   nth_error el (Z.to_nat i) = Some e →
   ▷ WP e @ E {{ Φ }} ⊢ WP Case (Lit $ LitInt i) el @ E {{ Φ }}.
 Proof.
-  intros. rewrite -(wp_lift_pure_det_head_step (Case _ _) e None) ?right_id //.
-  intros; inv_head_step; auto.
+  iIntros {??} "?". iApply wp_lift_pure_det_head_step; eauto.
+  by intros; inv_head_step; eauto. iNext. by iFrame.
 Qed.
 End lifting.
